
equation \ref{eq-1} is 

$$ \begin{align}
\max_{\mathbf{E}(t), \mathbf{F}(t), \mathbf{U}(t)} \quad & \mathcal{M}_t \left[\mathbf{Y}(t), \mathbf{X}(t), \mathbf{B}^{\mathrm{p}}(t), \mathbf{A}^{\mathrm{p}}(t) \right] \\
& = - \mathbf{H}(t)^{\top} \mathbf{Q} - \left[\mathbf{G}^{+}(t) + \mathbf{G}^{-}(t) \right]^{\top} \mathbf{O} \\
& - \mathbf{U}(t)^{\top} \mathbf{R} + l \left[ \mathbf{E}^{+}(t)^{\top} \mathbf{B}^{\mathrm{p}}(t) - \mathbf{E}^{-}(t)^{\top} \mathbf{A}^{\mathrm{p}}(t) \right] \\
& - [\mathbf{F}^{+}(t) + \mathbf{F}^{-}(t)]^{\top} \mathbf{P} \\
\text{s.t.} \quad & \mathbf{w}_{i+k+1}(t) = \mathbf{A} \mathbf{w}_{i+k}(t) + \mathbf{B} \mathbf{u}_{i+k}(t) \quad \forall k \in K \\
& \mathbf{v}_{i+k}(t) = \mathbf{C} \mathbf{w}_{i+k}(t) + \mathbf{D} \mathbf{u}_{i+k}(t) \quad \forall k \in K \\
& \mathbf{v}_{\text{min}} \leq \mathbf{v}_{i+k}(t) \leq \mathbf{v}_{\text{max}} \quad \forall k \in K \\
& \mathbf{u}_{\text{min}} \leq \mathbf{u}_{i+k}(t) \leq \mathbf{u}_{\text{max}} \quad \forall k \in K \\
& - \mathbf{u}_{\Delta} \leq \mathbf{u}_{i+k+1}(t) - \mathbf{u}_{i+k}(t) \leq \mathbf{u}_{\Delta} \quad \forall k \in K_{-} \\
& \mathbf{E}^{+}(t) \geq 0 \quad \\
& \mathbf{E}^{+}(t) \geq \mathbf{E}(t)  \\
& \mathbf{E}^{-}(t) \geq 0 \\
& \mathbf{E}^{-}(t) \geq - \mathbf{E}(t) \\
& \mathbf{H}(t) \geq 0 \\
& \mathbf{H}(t) \geq \mathbf{Y}(t) + \mathbf{E}(t) - \mathbf{U}(t) \tag{1} \\
& \mathbf{G}^{+}(t) \geq 0 \\
& \mathbf{G}^{+}(t) \geq \mathbf{V}(t) - \mathbf{X}(t) - \mathbf{F}(t) \tag{2} \\
& \mathbf{G}^{-}(t) \geq 0 \\
& \mathbf{G}^{-}(t) \geq \mathbf{X}(t) + \mathbf{F}(t) - \mathbf{V}(t) \tag{3} \\
& \mathbf{F}^{+}(t) \geq 0 \quad \\
& \mathbf{F}^{+}(t) \geq \mathbf{F}(t)  \\
& \mathbf{F}^{-}(t) \geq 0 \\
& \mathbf{F}^{-}(t) \geq - \mathbf{F}(t) \\
& \mathbf{E}(t) \in \mathbb{R}^{\kappa} \\
& \mathbf{F}(t) \in \mathbb{R}^{\kappa} \\
& \mathbf{U}(t) \in \mathbb{R}^{\kappa}_{+}
\end{align} $$



